src/FcEtt/ett_ind.v
@@ -452,7 +452,8 @@ Ltac gather_atoms ::=
   let D8 := gather_atoms_with (fun x => fv_co_co_constraint x) in
   let D9 := gather_atoms_with (fun x => fv_co_co_sort x) in
   let D10 := gather_atoms_with (fun x => fv_co_co_brs x) in
-  constr:(A \u B \u C1 \u D1 \u D2 \u D3 \u D4 \u D5 \u D6 \u D7 \u D8 \u D9 \u D10).
+  let D11 := gather_atoms_with (fun x : econtext => dom x) in
+  constr:(A \u B \u C1 \u D1 \u D2 \u D3 \u D4 \u D5 \u D6 \u D7 \u D8 \u D9 \u D10 \u D11).
 
 
 (* ----------------------------------------------------- *)
